Demo: re-defined the safety interfaces for composition; fixed the proofs of linked_list

rustdemo/HashMapCommon.v
@@ -11,6 +11,8 @@ Require Import Events.
 Require Import Invariant Smallstep SmallstepLinkingSafe.
 Require Import HashMap.
 Require Import LinkedList RustOp Rusttypes Rustlight Rustlightown.
+Require Import LanguageInterface.
+Require Import MoveCheckingDomain.
 
 Local Open Scope error_monad_scope.
 Import ListNotations.
@@ -44,23 +46,154 @@ Remark starNf_step_right ge: forall n s t t1 s' t2 s'',
     starNf ge n s t1 s' -> step ge s' t2 s'' -> t = t1 ** t2 ->
     numf s' = numf s'' ->
     starNf ge (S n) s t s''.
-Admitted.
+Proof.
+  induction n; intros until s''; intros STAR STEP TC NUM.
+  - inv STAR. econstructor; eauto. econstructor.
+    rewrite E0_right. reflexivity.
+  - inv STAR. econstructor. eauto.
+    eapply IHn; eauto. eapply Eapp_assoc. auto.
+Qed.
 
 End CLOSURES.
 
 
-(* The kripke world used in proving partial safety *)
-Record hmap_world :=
-  { 
-    hmap_callee: ident + ident;         (* remember the called
-    function (inl is in linked_list and inr is in the C module) to
-    specify the post condition when returning the current module. How
-    to generalize it? *)
-    hmap_senv: Genv.symtbl;
-    hmap_hash_range : int }.
+(* (* The kripke world used in proving partial safety *) *)
+(* Record hmap_world := *)
+(*   {  *)
+(*     hmap_callee: ident + ident;         (* remember the called *)
+(*     function (inl is in linked_list and inr is in the C module) to *)
+(*     specify the post condition when returning the current module. How *)
+(*     to generalize it? *) *)
+(*     hmap_senv: Genv.symtbl; *)
+(*     hmap_hash_range : int }. *)
 
 
-(* pre-post conditions of hash function *)
+(* (* pre-post conditions of hash function *) *)
+
+(* Inductive hash_pre_cond_args r : list Values.val -> Prop := *)
+(* | hash_pre_cond_args_intro: forall k *)
+(*     (GTZ: Int.ltu Int.zero r = true) *)
+(*     (CASTED1: val_casted (Vint k) type_int32s) *)
+(*     (CASTED1: val_casted (Vint r) type_int32u), *)
+(*     hash_pre_cond_args r [Vint k; Vint r]. *)
+
+(* Inductive hash_post_cond_retv range : Values.val -> Prop := *)
+(* | hash_post_cond_retv_intro: forall r     *)
+(*     (INRAN: Int.ltu r range = true), *)
+(*     hash_post_cond_retv range (Vint r). *)
+
+(* (** Pre/Post-conditions parameterized by the function name *) *)
+(* Definition linked_list_args_pre_conds r (f: ident) : list Values.val -> Prop := *)
+(*   if ident_eq f hash then *)
+(*     hash_pre_cond_args r *)
+(*   else fun _ => True. *)
+
+(* Definition linked_list_retv_post_conds r (f: ident) : Values.val -> Prop := *)
+(*   if ident_eq f hash then *)
+(*     hash_post_cond_retv r *)
+(*   else fun _ => True. *)
+
+(* (* Initial preservation and progress *) *)
+(* Inductive vq_hash_map (w: hmap_world) : rust_query -> Prop := *)
+(* (* incoming call of linked_list (i.e., the outgoing call of hmap) *) *)
+(* | vq_hash_map_intro1: forall b f targs tres tcc vargs m orgs rels fid *)
+(*     (FINDF: Genv.find_funct_ptr (globalenv w.(hmap_senv) linked_list_mod) b = Some (Internal f)) *)
+(*     (NFHMAP: Genv.is_internal (Genv.globalenv w.(hmap_senv) hash_map_prog) (Vptr b Ptrofs.zero) = false) *)
+(*     (TYF: type_of_function f = Tfunction orgs rels targs tres tcc) *)
+(*     (NOTDROP: fn_drop_glue f = None) *)
+(*     (CASTED: val_casted_list vargs targs) *)
+(*     (SYM: Genv.invert_symbol w.(hmap_senv) b = Some fid) *)
+(*     (PRECOND: linked_list_args_pre_conds w.(hmap_hash_range) fid vargs) *)
+(*     (FIDEQ: w.(hmap_callee) = inl fid) *)
+(*     (LEN: length_of_args fid = length vargs), *)
+(*     vq_hash_map w (rsq (Vptr b Ptrofs.zero) (mksignature orgs rels (type_list_of_typelist targs) tres tcc (prog_comp_env linked_list_mod)) vargs m) *)
+(* (* outgoing call (which is specific to the definition of the C *)
+(* module..). For now, we only support calling the process function from *)
+(* Rust side. Other functions in the C module are static. *) *)
+(* | vq_hash_map_intro2: forall b f targs tres tcc vargs m orgs rels fid *)
+(*     (FINDF: Genv.find_funct_ptr (Genv.globalenv w.(hmap_senv) hash_map_prog) b = Some (Ctypes.Internal f)) *)
+(*     (NFLINK: Genv.is_internal (globalenv w.(hmap_senv) linked_list_mod) (Vptr b Ptrofs.zero)= false) *)
+(*     (TYF: Clight.type_of_function f = Ctypes.Tfunction (to_ctypelist targs) (to_ctype tres) tcc) *)
+(*     (CASTED: val_casted_list vargs targs) *)
+(*     (SYM: Genv.invert_symbol w.(hmap_senv) b = Some fid) *)
+(*     (** we only permit process function be called from Rust *) *)
+(*     (ONLYPROCESS: fid = process) *)
+(*     (TARGSEQ: targs = (Tcons (Tbox type_int32s) Tnil)) *)
+(*     (TRESEQ: tres = Tbox type_int32s) *)
+(*     (PRECOND: linked_list_args_pre_conds w.(hmap_hash_range) fid vargs) *)
+(*     (FIDEQ: w.(hmap_callee) = inr fid) *)
+(*     (LEN: length_of_args fid = length vargs), *)
+(*     vq_hash_map w (rsq (Vptr b Ptrofs.zero) (mksignature orgs rels (type_list_of_typelist targs) tres tcc (prog_comp_env linked_list_mod)) vargs m). *)
+    
+(* Inductive vr_hash_map (w: hmap_world) : rust_reply -> Prop := *)
+(* (* return from linked_list module *) *)
+(* | vr_hash_map_intro1: forall v m fid *)
+(*     (FIDEQ: w.(hmap_callee) = inl fid) *)
+(*     (POSTCOND: linked_list_retv_post_conds w.(hmap_hash_range) fid v), *)
+(*     vr_hash_map w (rsr v m) *)
+(* (* return from hash_map module *) *)
+(* | vr_hash_map_intro2: forall v m fid *)
+(*     (FIDEQ: w.(hmap_callee) = inr fid), *)
+(*     vr_hash_map w (rsr v m) *)
+(* . *)
+
+(* Definition wf_senv se := *)
+(*   forall id, *)
+(*     if in_dec ident_eq id ((prog_defs_names linked_list_mod) ++ (prog_defs_names hash_map_prog)) *)
+(*     then *)
+(*       exists b, Genv.find_symbol se id = Some b *)
+(*     else True. *)
+
+(* Definition hmap_inv : invariant li_rs := *)
+(*   {| inv_world := hmap_world; *)
+(*     symtbl_inv w se := w.(hmap_senv) = se *)
+(*                        /\ wf_senv se; *)
+(*     query_inv w q := vq_hash_map w q; *)
+(*     reply_inv w r := vr_hash_map w r |}. *)
+
+(** Safety interfaces for hmap.c and list.rs:
+
+    ⟦hmap.c⟧ ⊩ {find_process ↦ ⊤, hash ↦ P} ⋅ I_rs⋅R_rc
+             ↠ {process ↦ ⊤⋅I_rs⋅R_rc, hmap_process ↦ Q}
+
+    ⟦hmap.s⟧ ⊩ {find_process ↦ ⊤, hash ↦ P} ⋅ I_rs⋅R_rc⋅R_ca
+             ↠ {process ↦ ⊤⋅I_rs⋅R_rc, hmap_process ↦ Q} ⋅ R_ca
+
+    ⟦list.rs⟧ ⊩ {process ↦ ⊤, hmap_process ↦ ⊥}
+             ↠ {find_process ↦ ⊤, hash ↦ P}
+
+    ⟦list.s⟧ ⊩ {process ↦ ⊤, hmap_process ↦ ⊥} ⋅ (I_rs⋅R_ra) ⇒ (I_rs⋅R_rc⋅R_ca)
+             ↠ {find_process ↦ ⊤, hash ↦ P} ⋅ I_rs⋅R_ra
+
+    ⟦list.s⟧ ⊩ {process ↦ ⊤⋅I_rs⋅R_rc, hmap_process ↦ Q} ⋅ R_ca
+             ↠ {find_process ↦ ⊤, hash ↦ P} ⋅ I_rs⋅R_ra
+             
+    Note that list.rs impossibly calls hmap_process, so the ⊥
+    interface can be refined to anything.
+
+    {find_process ↦ ⊤, hash ↦ P}: hmap_ext_inv
+
+    {process ↦ ⊤⋅I_rs⋅R_rc, hmap_process ↦ Q}: hmap_int_inv
+
+    {process ↦ ⊤, hmap_process ↦ ⊥}: list_ext_inv
+ *)
+
+
+Record hmap_world_ext :=
+  {
+    hmap_callee_ext: ident; (* remember the called function *)
+    hmap_senv_ext: Genv.symtbl;
+    hmap_hash_range_ext : int }.
+
+Definition wf_senv se :=
+  forall id,
+    if in_dec ident_eq id (prog_defs_names hash_map_prog ++ prog_defs_names linked_list_mod)
+    then
+      exists b, Genv.find_symbol se id = Some b
+    else True.
+
+
+(** Pre- and Post- conditions for hash function *)
 
 Inductive hash_pre_cond_args r : list Values.val -> Prop :=
 | hash_pre_cond_args_intro: forall k
@@ -70,20 +203,201 @@ Inductive hash_pre_cond_args r : list Values.val -> Prop :=
     hash_pre_cond_args r [Vint k; Vint r].
 
 Inductive hash_post_cond_retv range : Values.val -> Prop :=
-| hash_post_cond_retv_intro: forall r    
+| hash_post_cond_retv_intro: forall r
     (INRAN: Int.ltu r range = true),
     hash_post_cond_retv range (Vint r).
 
-(** Pre/Post-conditions parameterized by the function name *)
-Definition linked_list_args_pre_conds r (f: ident) : list Values.val -> Prop :=
-  if ident_eq f hash then
-    hash_pre_cond_args r
-  else fun _ => True.
+Inductive vq_hash (w: hmap_world_ext) : rust_query -> Prop :=
+(* incoming call of linked_list (i.e., the outgoing call of hmap) *)
+| vq_hash_intro: forall vf targs tres tcc vargs m orgs rels
+    (* For safety of initial_state *)
+    (FINDF: Genv.find_funct (globalenv w.(hmap_senv_ext) linked_list_mod) vf = Some (Internal hash_func))
+    (CASTED: val_casted_list vargs targs)
+    (TYF: type_of_function hash_func = Tfunction orgs rels targs tres tcc)
+    (PRECOND: hash_pre_cond_args w.(hmap_hash_range_ext) vargs)
+    (CALLEE: hmap_callee_ext w = hash),
+    vq_hash w (rsq vf (mksignature orgs rels (type_list_of_typelist targs) tres tcc (prog_comp_env linked_list_mod)) vargs m).
 
-Definition linked_list_retv_post_conds r (f: ident) : Values.val -> Prop :=
-  if ident_eq f hash then
-    hash_post_cond_retv r
-  else fun _ => True.
+Inductive vr_hash (w: hmap_world_ext) : rust_reply -> Prop :=
+(* return from linked_list module *)
+| vr_hash_intro: forall v m
+    (POSTCOND: hash_post_cond_retv w.(hmap_hash_range_ext) v),
+    vr_hash w (rsr v m).
+
+Inductive vq_find (w: hmap_world_ext) : rust_query -> Prop :=
+(* incoming call of linked_list (i.e., the outgoing call of hmap) *)
+| vq_find_intro: forall vf targs tres tcc vargs m orgs rels
+    (* For safety of initial_state *)
+    (FINDF: Genv.find_funct (globalenv w.(hmap_senv_ext) linked_list_mod) vf = Some (Internal find_func))
+    (CASTED: val_casted_list vargs targs)
+    (TYF: type_of_function find_func = Tfunction orgs rels targs tres tcc)
+    (LEN: length vargs = 2%nat)
+    (CALLEE: hmap_callee_ext w = find),
+    vq_find w (rsq vf (mksignature orgs rels (type_list_of_typelist targs) tres tcc (prog_comp_env linked_list_mod)) vargs m).
+
+
+
+(** External interface for hmap.c  *)
+Definition rsq_inv_hmap_ext (w: hmap_world_ext) (q: rust_query) (fid: ident) : Prop :=
+  if ident_eq fid find then
+    (* Although find does not have pre-and post conditions, we need to
+    consider the length of arguements and the signature *)
+    vq_find w q
+  else if ident_eq fid hash then
+         vq_hash w q 
+       else False.
+
+Definition rsr_inv_hmap_ext (w: hmap_world_ext) (r: rust_reply) (fid: ident) : Prop :=
+  if ident_eq fid find then
+    True
+  else if ident_eq fid hash then
+         vr_hash w r 
+       else False.
+
+
+(* Pre-conditions of rust query composed of the conditions of each
+function *)
+Definition rsq_inv {W: Type} (w: W) (q: rust_query) se (fn_pred: W -> rust_query -> ident -> Prop) : Prop :=
+  match rsq_vf q with
+  | Vptr b ofs =>
+      if Ptrofs.eq_dec ofs Ptrofs.zero then
+        match Genv.invert_symbol se b with
+        | Some id =>
+            fn_pred w q id
+        | _ => False
+        end
+      else
+        False
+  | _ => False
+  end.
+
+Definition rsr_inv {W: Type} (w: W) (r: rust_reply) callee (fn_pred: W -> rust_reply -> ident -> Prop) : Prop :=
+  fn_pred w r callee.
+  
+(* Safety interfaces for external calls of hmap.c, i.e., {find_process ↦ ⊤, hash ↦ P} *)
+Definition hmap_ext_inv : invariant li_rs :=
+  {| inv_world := hmap_world_ext;
+    symtbl_inv w se := w.(hmap_senv_ext) = se
+                       (* wf_xx_senv is used to ensure the safety of
+                       function call (see eval_Eglobal) *)
+                       /\ wf_senv se;
+    query_inv w q := rsq_inv w q (hmap_senv_ext w) rsq_inv_hmap_ext;
+    reply_inv w r := rsr_inv w r (hmap_callee_ext w) rsr_inv_hmap_ext|}.
+
+
+(* External interface of linked list *)
+
+Record list_world_ext :=
+  {
+    list_callee_ext: ident; (* remember the called function *)
+    list_senv_ext: Genv.symtbl;
+  }.
+
+
+
+Inductive vq_process (w: list_world_ext) : rust_query -> Prop :=
+| vq_process_intro: forall vf targs tres tcc vargs m orgs rels
+    (* For safety of initial_state *)
+    (FINDF: Genv.find_funct (Genv.globalenv w.(list_senv_ext) hash_map_prog) vf = Some (Ctypes.Internal process_func))
+    (TYF: Clight.type_of_function process_func = Ctypes.Tfunction (to_ctypelist targs) (to_ctype tres) tcc)
+    (CASTED: val_casted_list vargs targs)
+    (TARGSEQ: targs = (Tcons (Tbox type_int32s) Tnil))
+    (TRESEQ: tres = Tbox type_int32s)    
+    (LEN: length vargs = 1%nat)
+    (CALLEE: list_callee_ext w = process),
+    vq_process w (rsq vf (mksignature orgs rels (type_list_of_typelist targs) tres tcc (prog_comp_env linked_list_mod)) vargs m).
+
+
+Definition rsq_inv_list_ext (w: list_world_ext) (q: rust_query) (fid: ident) : Prop :=
+  if ident_eq fid process then
+    (* process ↦ ⊤. We need to consider the length of arguments and signature *)
+    vq_process w q
+  else if ident_eq fid hmap_process then
+         (* {hmap_process ↦ ⊥} *)
+         False
+       else False.
+
+Definition rsr_inv_list_ext (w: list_world_ext) (r: rust_reply) (fid: ident) : Prop :=
+  if ident_eq fid process then
+    (* process ↦ ⊤ *)
+    True
+  else if ident_eq fid hmap_process then
+         (* {hmap_process ↦ ⊥} *)
+         False
+       else False.
+
+(* {process ↦ ⊤, hmap_process ↦ ⊥}  *)
+Definition list_ext_inv: invariant li_rs := 
+  {| inv_world := list_world_ext;
+    symtbl_inv w se := w.(list_senv_ext) = se
+                       (* wf_senv is used to ensure the safety of
+                       function call in C and Rust sides (see eval_Eglobal) *)
+                       /\ wf_senv se;
+    query_inv w q := rsq_inv w q (list_senv_ext w) rsq_inv_list_ext;
+    reply_inv w r := rsr_inv w r (list_callee_ext w) rsr_inv_list_ext|}.
+
+(* Incoming interface for hmap. *)
+
+Record hmap_world_int :=
+  {
+    hmap_list_ext: list_world_ext;
+    hmap_rs_own: rs_own_world;
+  }.
+
+Local Open Scope inv_scope.
+
+Definition cq_inv_hmap_int (w: hmap_world_int) (q: c_query) (fid: ident) : Prop :=
+  if ident_eq fid process then
+    (* process ↦ ⊤⋅I_rs⋅R_rc. ⊤ requires us to consider the length of
+    argument and signature *)
+    query_inv ((list_ext_inv @@ rs_own) @! cc_rust_c)
+      (w.(hmap_list_ext), (w.(hmap_list_ext).(list_senv_ext), w.(hmap_rs_own)), tt) q
+  else if ident_eq fid hmap_process then
+         (* TODO *)
+         True
+       else False.
+
+Definition cr_inv_hmap_int (w: hmap_world_int) (r: c_reply) (fid: ident) : Prop :=
+  if ident_eq fid process then
+    (* process ↦ ⊤⋅I_rs⋅R_rc *)
+    reply_inv ((list_ext_inv @@ rs_own) @! cc_rust_c)
+      (w.(hmap_list_ext), (w.(hmap_list_ext).(list_senv_ext), w.(hmap_rs_own)), tt) r
+  else if ident_eq fid hmap_process then
+         (* TODO *)
+         True
+       else False.
+
+(* Pre-conditions of rust query composed of the conditions of each
+function *)
+Definition cq_inv {W: Type} (w: W) (q: c_query) se (fn_pred: W -> c_query -> ident -> Prop) : Prop :=
+  match cq_vf q with
+  | Vptr b ofs =>
+      if Ptrofs.eq_dec ofs Ptrofs.zero then
+        match Genv.invert_symbol se b with
+        | Some id =>
+            fn_pred w q id
+        | _ => False
+        end
+      else
+        False
+  | _ => False
+  end.
+
+Definition cr_inv {W: Type} (w: W) (r: c_reply) callee (fn_pred: W -> c_reply -> ident -> Prop) : Prop :=
+  fn_pred w r callee
+.
+
+(* Safety interfaces for incoming calls of hmap.c,
+   i.e., {process ↦ ⊤⋅I_rs⋅R_rc, hmap_process ↦ Q} *)
+Definition hmap_int_inv : invariant li_c :=
+  {| inv_world := hmap_world_int;
+    symtbl_inv w se := (list_senv_ext (hmap_list_ext w)) = se
+                       (* wf_xx_senv is used to ensure the safety of
+                       function call (see eval_Eglobal) *)
+                       /\ wf_senv se;
+    query_inv w q := cq_inv w q (list_senv_ext (hmap_list_ext w)) cq_inv_hmap_int;
+    reply_inv w r := cr_inv w r (list_callee_ext (hmap_list_ext w)) cr_inv_hmap_int|}.
+
 
 Definition length_of_args (f: ident) : nat :=
   if ident_eq f find then
@@ -94,62 +408,4 @@ Definition length_of_args (f: ident) : nat :=
     else if ident_eq f process then
            1
   else O.
-
-(* Initial preservation and progress *)
-Inductive vq_hash_map (w: hmap_world) : rust_query -> Prop :=
-(* incoming call of linked_list (i.e., the outgoing call of hmap) *)
-| vq_hash_map_intro1: forall b f targs tres tcc vargs m orgs rels fid
-    (FINDF: Genv.find_funct_ptr (globalenv w.(hmap_senv) linked_list_mod) b = Some (Internal f))
-    (NFHMAP: Genv.is_internal (Genv.globalenv w.(hmap_senv) hash_map_prog) (Vptr b Ptrofs.zero) = false)
-    (TYF: type_of_function f = Tfunction orgs rels targs tres tcc)
-    (NOTDROP: fn_drop_glue f = None)
-    (CASTED: val_casted_list vargs targs)
-    (SYM: Genv.invert_symbol w.(hmap_senv) b = Some fid)
-    (PRECOND: linked_list_args_pre_conds w.(hmap_hash_range) fid vargs)
-    (FIDEQ: w.(hmap_callee) = inl fid)
-    (LEN: length_of_args fid = length vargs),
-    vq_hash_map w (rsq (Vptr b Ptrofs.zero) (mksignature orgs rels (type_list_of_typelist targs) tres tcc (prog_comp_env linked_list_mod)) vargs m)
-(* outgoing call (which is specific to the definition of the C
-module..). For now, we only support calling the process function from
-Rust side. Other functions in the C module are static. *)
-| vq_hash_map_intro2: forall b f targs tres tcc vargs m orgs rels fid
-    (FINDF: Genv.find_funct_ptr (Genv.globalenv w.(hmap_senv) hash_map_prog) b = Some (Ctypes.Internal f))
-    (NFLINK: Genv.is_internal (globalenv w.(hmap_senv) linked_list_mod) (Vptr b Ptrofs.zero)= false)
-    (TYF: Clight.type_of_function f = Ctypes.Tfunction (to_ctypelist targs) (to_ctype tres) tcc)
-    (CASTED: val_casted_list vargs targs)
-    (SYM: Genv.invert_symbol w.(hmap_senv) b = Some fid)
-    (** we only permit process function be called from Rust *)
-    (ONLYPROCESS: fid = process)
-    (TARGSEQ: targs = (Tcons (Tbox type_int32s) Tnil))
-    (TRESEQ: tres = Tbox type_int32s)
-    (PRECOND: linked_list_args_pre_conds w.(hmap_hash_range) fid vargs)
-    (FIDEQ: w.(hmap_callee) = inr fid)
-    (LEN: length_of_args fid = length vargs),
-    vq_hash_map w (rsq (Vptr b Ptrofs.zero) (mksignature orgs rels (type_list_of_typelist targs) tres tcc (prog_comp_env linked_list_mod)) vargs m).
-    
-Inductive vr_hash_map (w: hmap_world) : rust_reply -> Prop :=
-(* return from linked_list module *)
-| vr_hash_map_intro1: forall v m fid
-    (FIDEQ: w.(hmap_callee) = inl fid)
-    (POSTCOND: linked_list_retv_post_conds w.(hmap_hash_range) fid v),
-    vr_hash_map w (rsr v m)
-(* return from hash_map module *)
-| vr_hash_map_intro2: forall v m fid
-    (FIDEQ: w.(hmap_callee) = inr fid),
-    vr_hash_map w (rsr v m)
-.
-
-Definition wf_senv se :=
-  forall id,
-    if in_dec ident_eq id ((prog_defs_names linked_list_mod) ++ (prog_defs_names hash_map_prog))
-    then
-      exists b, Genv.find_symbol se id = Some b
-    else True.
-
-Definition hmap_inv : invariant li_rs :=
-  {| inv_world := hmap_world;
-    symtbl_inv w se := w.(hmap_senv) = se
-                       /\ wf_senv se;
-    query_inv w q := vq_hash_map w q;
-    reply_inv w r := vr_hash_map w r |}.
-
+  
